Merkle trees: 64-bit indices (but 32-bit indexed tree); added cleaner C header interface; added some basic serialization.

secure_api/merkle_tree/MerkleTree.h
@@ -1,0 +1,157 @@
+/* Copyright (c) INRIA and Microsoft Corporation. All rights reserved.
+   Licensed under the Apache 2.0 License. */
+
+#ifndef _MERKLE_TREE_H_
+#define _MERKLE_TREE_H_
+
+#ifdef __cplusplus
+extern "C" {
+#endif
+
+#include "stdint.h"
+
+extern hash_vec;
+extern merkle_tree;
+
+typedef uint8_t *hash;
+typedef merkle_tree *mt_p;
+typedef hash_vec *path;
+
+/* Utilities */
+
+extern hash init_hash();
+extern void free_hash(hash h);
+
+extern path init_path();
+extern void free_path(path p);
+extern void clear_path(path p);
+
+/** Construction */
+extern merkle_tree mt_create(hash init);
+
+/** Destrcution */
+extern void mt_free(merkle_tree mt);
+
+/* Insertion
+ *
+ * @param[in]  mt  The Merkle tree
+ * @param[in]  v   The tree does not take ownership of the hash, it makes a copy
+ *                 of its content.
+ *
+ * Note: The content of the hash will be overwritten with an arbitrary value.
+ */
+extern void mt_insert(merkle_tree mt, hash v);
+
+/** Precondition predicate for mt_insert */
+extern bool mt_insert_pre(merkle_tree mt, hash v);
+
+
+/** Getting the Merkle root
+ *
+ * @param[in]  mt   The Merkle tree
+ * @param[out] root The Merkle root returned as a hash pointer
+ */
+extern void mt_get_root(merkle_tree mt, hash root);
+
+/** Precondition predicate for mt_get_root */
+extern vool mt_get_root_pre(merkle_tree mt, hash root);
+
+
+/** Getting a Merkle path
+ *
+ * @param[in]  mt   The Merkle tree
+ * @param[in]  idx  The index of the target hash
+ * @param[out] root The Merkle root
+ * @param[out] path A resulting Merkle path that contains the leaf hash.
+ *
+ * @return The number of elements in the tree
+ *
+ * Notes:
+ * - The resulting path contains pointers to hashes in the tree, not copies of
+ *   the hash values.
+ * - idx must be within the currently held indices in the tree (past the
+ *   last flush index).
+ */
+extern uint32_t mt_get_path(merkle_tree mt, uint64_t idx, hash root, hash *path);
+
+/** Precondition predicate for mt_get_path */
+extern bool mt_get_path_pre(merkle_tree mt, uint64_t idx, hash root, hash *path);
+
+
+/** Flush the Merkle tree
+ *
+ * @param[in]  mt   The Merkle tree
+ */
+extern void mt_flush(merkle_tree mt);
+
+/** Precondition predicate for mt_flush */
+extern bool mt_flush_pre(merkle_tree mt);
+
+
+/** Flush the Merkle tree up to a given index
+ *
+ * @param[in]  mt   The Merkle tree
+ * @param[in]  idx The index up to which to flush the tree
+ */
+extern void mt_flush_to(merkle_tree mt, uint64_t idx);
+
+/** Precondition predicate for mt_flush_to */
+extern bool mt_flush_to_pre(merkle_tree mt, uint64_t idx);
+
+
+/** Client-side verification
+ *
+ * @param[in]  mt   The Merkle tree
+ * @param[in]  tgt  The index of the target hash
+ * @param[in]  max  The maximum index + 1 of the tree when the path was generated
+ * @param[in]  path The Merkle path to verify
+ * @param[in]  root
+ *
+ * @return true if the verification succeeded, false otherwise
+ *
+ * Note: max - tgt must be less than 2^32.
+ */
+extern bool mt_verify(merkle_tree mt, uint64_t tgt, uint64_t max, hash *path, hash root);
+
+/** Precondition predicate for mt_verify */
+extern bool mt_verify_pre(merkle_tree mt, uint64_t tgt, uint64_t max, hash *path, hash root);
+
+
+/** Serialization size
+ *
+ * @param[in]  mt   The Merkle tree
+ *
+ * @return the number of bytes required to serialize the tree
+ */
+extern uint32_t mt_serialize_size(merkle_tree mt);
+
+
+/** Serialization
+ *
+ * @param[in]  mt   The Merkle tree
+ * @param[out] buf  The buffer to serialize the tree into
+ *
+ * @return the number of bytes written
+ *
+ * Note: buf must be a buffer of size mt_serialize_size(mt) or larger.
+ */
+extern uint32_t mt_serialize(merkle_tree mt, char *buf);
+
+
+/** Deserialization
+ *
+ * @param[in]  buf  The buffer to deserialize the tree from
+ * @param[out] mt   The Merkle tree
+ *
+ * @return true if the deserialization succeeded, false otherwise
+ *
+ * Note: buf must be a buffer of size mt_serialize_size(mt) or larger.
+ */
+extern bool mt_deserialize(const char *buf, merkle_tree mt);
+
+
+#ifdef __cplusplus
+}
+#endif
+
+#endif /* _MERKLE_TREE_H_ */
